Abstract env check  (#671)
* mv PCUICEqualityDec and abstract over Σ

* fix remove of tPrim

* set up abstract_env

* adapt safereduce

* guard condition in Prop and generalize wf_fixpoint

* remove graph from error messages

* adapt safereduce

* adapt typechecker

* fix abstract impl

* fix plugin in Extraction

* pointwise definition of correctness in abstract_impl

* generalize reflection and proper lemmas for EqualityDec

* adapt typechecker

* WIP proving optim_impl is correct

* make error monads abstract over environment and graph

* adapt typechecker

* add wfEnvImpl

* expand wfEnv for safechecker

* add missing definitions in wfUniverses

* adapt upto typechecker

* expand equality dec

* first pass on safechecker

* complete definition of abstract_env_prop

* provide implementations of abstract_env

* adapt conversion and typehcecker

* remove unused function from interface

* add abstract_env_empty

* fix todos in SafeConversion

* finish remaining todos in SafeConversion

* adapt SafeTemplateChecker

* adapt Extraction

* fix plugin

* adapt erasure

* the safechecker does not compute anymore  in Coq

* fix Global in SafeChecker

* reorder ml files

* add lzero to enironment instead of removing

* remove ml/mli from git

* add test-suite and translations to `make all`

* fix after rebase

* fix link to guard_impl

* move require to header

* fix typing_correctness.v

template-coq/src/quoter.ml
@@ -206,7 +206,7 @@ struct
             (Univ.LSet.add p levels, Univ.Constraint.add (x, Univ.Eq, p) cstrs)) rest acc)
         eqs (levels, cstrs)
     in
-    let levels = Univ.LSet.remove Univ.Level.set levels in
+    let levels = Univ.LSet.add Univ.Level.set levels in
     let levels = Univ.LSet.remove Univ.Level.prop levels in
     let levels = Univ.LSet.remove Univ.Level.sprop levels in
     let cstrs = Univ.Constraint.remove (Univ.Level.prop, Univ.Lt, Univ.Level.set) cstrs in
