erasure/theories/EOptimizePropDiscr.v
@@ -8,7 +8,7 @@ From MetaCoq.PCUIC Require Import PCUICAst PCUICAstUtils
      PCUICCumulativity PCUICSR PCUICSafeLemmata
      PCUICValidity PCUICPrincipality PCUICElimination PCUICSN.
 
-From MetaCoq.SafeChecker Require Import PCUICWfEnv.
+From MetaCoq.SafeChecker Require Import PCUICWfEnvImpl.
      
 From MetaCoq.Erasure Require Import EAstUtils EArities Extract Prelim ErasureCorrectness EDeps EExtends
     ErasureFunction ELiftSubst.
